compiler/inference/proofs/type_dCanonScript.sml
@@ -6,28 +6,6 @@ val _ = new_theory "type_dCanon"
 
 (* TODO: move *)
 
-val nsMap_build_ctor_tenv = Q.store_thm("nsMap_build_ctor_tenv",
-  `∀ga g h tenvT tds ids.
-  LENGTH tds = LENGTH ids
-  ∧ (∀x. MEM x (MAP SND (FLAT (MAP (SND o SND) tds))) ⇒
-         MAP (type_name_subst tenvT) (ga x) = (g (MAP (type_name_subst tenvT) x)))
-  ⇒
-  nsMap (λ(tvs,ts,tid). (tvs, g ts, h tid)) (build_ctor_tenv tenvT tds ids) =
-  build_ctor_tenv tenvT (MAP (I ## I ## MAP (I ## ga)) tds) (MAP h ids)`,
-  ntac 3 gen_tac
-  \\ recInduct build_ctor_tenv_ind
-  \\ rw[build_ctor_tenv_def]
-  \\ rw[nsMap_nsAppend, MAP_REVERSE, MAP_MAP_o, o_DEF, UNCURRY, LAMBDA_PROD]
-  \\ AP_TERM_TAC
-  \\ AP_TERM_TAC
-  \\ AP_TERM_TAC
-  \\ rw[MAP_EQ_f]
-  \\ pairarg_tac \\ fs[]
-  \\ match_mp_tac EQ_SYM
-  \\ first_x_assum irule
-  \\ rw[MEM_MAP,EXISTS_PROD]
-  \\ metis_tac[]);
-
 val tenv_equiv_def = Define
   `tenv_equiv tenv1 tenv2 ⇔
      nsAll2 (λi v1 v2. v1 = v2) tenv1.t tenv2.t ∧
